coq/MorelloTests.v
@@ -52,9 +52,9 @@ Module test_cap_getters_and_setters.
   Program Definition flags2:Flags.t := exist _ [false; true; false; true; false; true; false; true] _. 
     Next Obligation. reflexivity. Defined.
     
-  Definition perm_Load : list bool := PermissionsBV.make_permissions [PermissionsBV.Load_perm].
-  Definition perm_Load_Store : list bool := PermissionsBV.make_permissions [PermissionsBV.Load_perm; PermissionsBV.Store_perm].
-  Definition perm_Load_Execute : list bool := PermissionsBV.make_permissions [PermissionsBV.Load_perm; PermissionsBV.Execute_perm].
+  Definition perm_Load : list bool := Permissions.make_permissions [Permissions.Load_perm].
+  Definition perm_Load_Store : list bool := Permissions.make_permissions [Permissions.Load_perm; Permissions.Store_perm].
+  Definition perm_Load_Execute : list bool := Permissions.make_permissions [Permissions.Load_perm; Permissions.Execute_perm].
   
   Example is_valid_test_1 :
     cap_is_valid c1 = true.
@@ -73,7 +73,7 @@ Module test_cap_getters_and_setters.
     Proof. reflexivity. Qed.
 
   Example value_test_1 : 
-    let value:AddressValueBV.t := AddressValueBV.of_Z 50 in
+    let value:AddressValue.t := AddressValue.of_Z 50 in
     value = cap_get_value (cap_set_value c1 value).
     Proof. reflexivity. Qed. 
 
@@ -83,28 +83,28 @@ Module test_cap_getters_and_setters.
   Example flags_test_2 : flags2 = cap_get_flags (cap_set_flags c1 flags2).
     Proof. vm_compute. reflexivity. Qed. 
   
-  Import PermissionsBV.
+  Import Permissions.
   
   Example permissions_test_1 : 
-    PermissionsBV.perm_Universal = cap_get_perms c1.
+    Permissions.perm_Universal = cap_get_perms c1.
     Proof. reflexivity. Qed.
 
   Example permissions_test_2 : 
-    let mask : PermissionsBV.t := list_bool_to_bv (perm_Load_Store) in
+    let mask : Permissions.t := list_bool_to_bv (perm_Load_Store) in
     list_bool_to_bv perm_Load_Store = cap_get_perms (cap_narrow_perms c1 mask).
     Proof. reflexivity. Qed.
 
   Example permissions_test_3 : 
-    let mask : PermissionsBV.t := list_bool_to_bv (perm_Load_Store) in
+    let mask : Permissions.t := list_bool_to_bv (perm_Load_Store) in
     let cap := (cap_narrow_perms c1 mask) in 
-    let mask : PermissionsBV.t := list_bool_to_bv (perm_Load_Execute) in
+    let mask : Permissions.t := list_bool_to_bv (perm_Load_Execute) in
     list_bool_to_bv perm_Load = cap_get_perms (cap_narrow_perms cap mask).
     Proof. vm_compute. reflexivity. Qed.
 
   Example permissions_test_4 : 
-    let mask : PermissionsBV.t := list_bool_to_bv ((make_permissions [Load_perm; Execute_perm])) in  
+    let mask : Permissions.t := list_bool_to_bv ((make_permissions [Load_perm; Execute_perm])) in  
     let capA := (cap_narrow_perms c1 mask) in     
-    let perms : PermissionsBV.t := PermissionsBV.perm_Universal in 
+    let perms : Permissions.t := Permissions.perm_Universal in 
     let perms := perm_clear_store_cap perms in 
     let perms := perm_clear_store perms in 
     let perms := perm_clear_global perms in 
@@ -121,8 +121,8 @@ Module test_cap_getters_and_setters.
     let perms := perm_clear_user3 perms in 
     let perms := perm_clear_user2 perms in 
     let perms := perm_clear_user1 perms in 
-    let perms := PermissionsBV.of_list ((PermissionsBV.to_list perms)) in
-    let capB := (cap_narrow_perms c1 (match perms with Some p => p | None => PermissionsBV.perm_Universal end)) in
+    let perms := Permissions.of_list ((Permissions.to_list perms)) in
+    let capB := (cap_narrow_perms c1 (match perms with Some p => p | None => Permissions.perm_Universal end)) in
     capA = capB.
     Proof. vm_compute. reflexivity. Qed.
 
@@ -130,32 +130,32 @@ Module test_cap_getters_and_setters.
     let user_perms_A : (list bool) := get_user_perms (cap_get_perms (cap_cU ())) in 
     let user_perms_A := [ nth 0 user_perms_A false; negb (nth 1 user_perms_A false);
                         nth 2 user_perms_A false; negb (nth 3 user_perms_A false) ] in 
-    let user_perms_B : PermissionsBV.t := 
+    let user_perms_B : Permissions.t := 
       perm_and_user_perms (cap_get_perms (cap_cU ())) user_perms_A in
       user_perms_A = [true; false; true; false] /\
       get_user_perms user_perms_B = user_perms_A.
     Proof. vm_compute. split. reflexivity. reflexivity. Qed. 
  
   Example eqb_and_narrow_perm_test_1 :
-    let mask : PermissionsBV.t := list_bool_to_bv (perm_Load_Store) in
+    let mask : Permissions.t := list_bool_to_bv (perm_Load_Store) in
     (c2 = (cap_narrow_perms c1 mask))%stdpp.
     Proof. vm_compute. reflexivity. Qed.
 
   Example bounds_representable_exactly_test_1 :
-    let bounds : BoundsBV.t := 
-      (Z_to_bv BoundsBV.bound_len 305402128, Z_to_bv BoundsBV.bound_len 305427248) in (* the bounds of c3, which we know is representable *) 
+    let bounds : Bounds.t := 
+      (Z_to_bv Bounds.bound_len 305402128, Z_to_bv Bounds.bound_len 305427248) in (* the bounds of c3, which we know is representable *) 
     cap_bounds_representable_exactly c4 bounds = true.
     Proof. reflexivity. Qed. 
       
   Example bounds_representable_exactly_test_2 :
-    let bounds : BoundsBV.t := 
-      (Z_to_bv BoundsBV.bound_len 305402128, Z_to_bv BoundsBV.bound_len 306427248) in (* now we changed the common part of the bounds *) 
+    let bounds : Bounds.t := 
+      (Z_to_bv Bounds.bound_len 305402128, Z_to_bv Bounds.bound_len 306427248) in (* now we changed the common part of the bounds *) 
     cap_bounds_representable_exactly c4 bounds = false.
     Proof. reflexivity. Qed. 
   
   Example narrow_exact_and_get_bounds_test_1 : 
     (* The bounds of capability c5 are         (0x0011111111110000, 0x00011111111117770). *)
-    let '(new_base,new_limit) := BoundsBV.of_Zs  (0x0011111111113330, 0x00011111111117440) in 
+    let '(new_base,new_limit) := Bounds.of_Zs  (0x0011111111113330, 0x00011111111117440) in 
     (* We can see new_bounds can be represented exactly from cap5: https://www.morello-project.org/capinfo?c=0x1%3Afb00000034473337%3A1011111111113333 *)
     let new_cap := cap_narrow_bounds_exact c5 (new_base,new_limit) in 
     let result := cap_get_bounds new_cap in 
@@ -203,62 +203,62 @@ Module test_cap_getters_and_setters.
     Proof. repeat ( split; try reflexivity ). Qed.
         
   Example alloc_cap_test_1 : 
-    let value := AddressValueBV.of_Z 1024 in 
-    let new_cap := alloc_cap value (AddressValueBV.of_Z 2048) in 
+    let value := AddressValue.of_Z 1024 in 
+    let new_cap := alloc_cap value (AddressValue.of_Z 2048) in 
     (cap_is_valid new_cap) /\ (cap_get_value new_cap) = value 
     /\ (cap_is_in_bounds new_cap) /\ (cap_is_sealed new_cap) = false 
     /\ (cap_get_seal new_cap) = SealType.Cap_Unsealed 
-    /\ (cap_get_perms new_cap) = PermissionsBV.perm_alloc
-    /\ (cap_get_bounds_ new_cap) = (BoundsBV.of_Zs (1024,3072), true).
+    /\ (cap_get_perms new_cap) = Permissions.perm_alloc
+    /\ (cap_get_bounds_ new_cap) = (Bounds.of_Zs (1024,3072), true).
     Proof. vm_compute. repeat (split; try reflexivity). Qed. 
   
   Example alloc_cap_test_2 : 
-    let value := AddressValueBV.of_Z 0xffffffffffffffff in (* 16 f's = the largest Value possible *)
-    let new_cap := alloc_cap value (AddressValueBV.of_Z 1) in 
+    let value := AddressValue.of_Z 0xffffffffffffffff in (* 16 f's = the largest Value possible *)
+    let new_cap := alloc_cap value (AddressValue.of_Z 1) in 
     (cap_is_valid new_cap) = true /\ (cap_get_value new_cap) = value 
     /\ (cap_is_in_bounds new_cap) /\ (cap_is_sealed new_cap) = false 
     /\ (cap_get_seal new_cap) = SealType.Cap_Unsealed 
-    /\ (cap_get_perms new_cap) = PermissionsBV.perm_alloc
-    /\ (cap_get_bounds_ new_cap) = (BoundsBV.of_Zs (0xffffffffffffffff,0x10000000000000000), true).
+    /\ (cap_get_perms new_cap) = Permissions.perm_alloc
+    /\ (cap_get_bounds_ new_cap) = (Bounds.of_Zs (0xffffffffffffffff,0x10000000000000000), true).
     Proof. vm_compute. repeat (split; try reflexivity). Qed. 
 
   Example alloc_cap_test_3 : 
-    let value := AddressValueBV.of_Z 0x10000000000000000 in (* 1 past the largest Value possible; it gets passed as just 0 *)
-    let new_cap := alloc_cap value (AddressValueBV.of_Z 1) in 
+    let value := AddressValue.of_Z 0x10000000000000000 in (* 1 past the largest Value possible; it gets passed as just 0 *)
+    let new_cap := alloc_cap value (AddressValue.of_Z 1) in 
     (cap_is_valid new_cap) = true 
     /\ (cap_is_in_bounds new_cap) = true (* it's in bounds bc these are (0,1) *)
     /\ (cap_is_sealed new_cap) = false /\ (cap_get_seal new_cap) = SealType.Cap_Unsealed 
-    /\ (cap_get_perms new_cap) = PermissionsBV.perm_alloc  
-    /\ (cap_get_bounds_ new_cap) <> (BoundsBV.of_Zs (0x10000000000000000,0x10000000000000001), true).
+    /\ (cap_get_perms new_cap) = Permissions.perm_alloc  
+    /\ (cap_get_bounds_ new_cap) <> (Bounds.of_Zs (0x10000000000000000,0x10000000000000001), true).
     Proof. vm_compute. repeat (split; try reflexivity). intros H. discriminate H. Qed.
 
   Example alloc_cap_test_4 : 
-    let value := AddressValueBV.of_Z 0xffffffffffffff in (* 14 f's *)
-    let new_cap := alloc_cap value (AddressValueBV.of_Z 0xfff) in (* this sends the limit above the max limit allowed *)
+    let value := AddressValue.of_Z 0xffffffffffffff in (* 14 f's *)
+    let new_cap := alloc_cap value (AddressValue.of_Z 0xfff) in (* this sends the limit above the max limit allowed *)
     (cap_is_invalid new_cap) /\ (cap_is_not_in_bounds new_cap)
     /\ (cap_is_sealed new_cap) = false /\ (cap_get_seal new_cap) = SealType.Cap_Unsealed 
-    /\ (cap_get_perms new_cap) = PermissionsBV.perm_alloc  
-    /\ (cap_get_bounds_ new_cap) <> (BoundsBV.of_Zs (0xffffffffffffff,0xfffffffffffffffff), true).
+    /\ (cap_get_perms new_cap) = Permissions.perm_alloc  
+    /\ (cap_get_bounds_ new_cap) <> (Bounds.of_Zs (0xffffffffffffff,0xfffffffffffffffff), true).
     Proof. vm_compute. repeat (split; try reflexivity). intro H. discriminate H. Qed.   
           
   Example alloc_fun_test_1 : 
-    let value := AddressValueBV.of_Z 1024 in 
+    let value := AddressValue.of_Z 1024 in 
     let new_cap := alloc_fun value in 
     (cap_is_valid new_cap) = true /\ (cap_get_value new_cap) = value 
       /\ (cap_is_sealed new_cap) = true /\ (cap_get_seal new_cap) = SealType.Cap_SEntry 
-      /\ (cap_get_perms new_cap) = PermissionsBV.perm_alloc_fun
-      /\ (cap_get_bounds_ new_cap) = (BoundsBV.of_Zs (1024,1026), true).
+      /\ (cap_get_perms new_cap) = Permissions.perm_alloc_fun
+      /\ (cap_get_bounds_ new_cap) = (Bounds.of_Zs (1024,1026), true).
     Proof. repeat (split; try reflexivity). Qed. 
 
   Example cap_is_null_derived_test_1 : 
     let new_cap := cap_c0 () in 
-    let new_cap := cap_set_value new_cap (AddressValueBV.of_Z 512) in 
+    let new_cap := cap_set_value new_cap (AddressValue.of_Z 512) in 
     (cap_is_null_derived new_cap) = true.
     Proof. vm_compute. reflexivity. Qed.
       
   Example cap_is_null_derived_test_2 : 
     let new_cap := cap_cU () in 
-    let new_cap := cap_set_value new_cap (AddressValueBV.of_Z 512) in 
+    let new_cap := cap_set_value new_cap (AddressValue.of_Z 512) in 
     (cap_is_null_derived new_cap) = false.
     Proof. vm_compute. reflexivity. Qed.
 
